code/bignum/Hacl.Spec.Bignum.Addition.fst
@@ -12,11 +12,11 @@ open Hacl.Spec.Lib
 
 #reset-options "--z3rlimit 50 --fuel 0 --ifuel 0"
 
-val bn_sub1_f: #t:limb_t -> #aLen:size_nat -> a:lbignum t aLen -> i:size_nat{i < aLen} -> c_in:carry t -> carry t & limb t
-let bn_sub1_f #t #aLen a i c_in = subborrow c_in a.[i] (uint #t 0)
+val bn_sub_carry_f: #t:limb_t -> #aLen:size_nat -> a:lbignum t aLen -> i:size_nat{i < aLen} -> c_in:carry t -> carry t & limb t
+let bn_sub_carry_f #t #aLen a i c_in = subborrow c_in a.[i] (uint #t 0)
 
-val bn_sub1: #t:limb_t -> #aLen:size_nat -> a:lbignum t aLen -> c_in:carry t -> tuple2 (carry t) (lbignum t aLen)
-let bn_sub1 #t #aLen a c_in = generate_elems aLen aLen (bn_sub1_f a) c_in
+val bn_sub_carry: #t:limb_t -> #aLen:size_nat -> a:lbignum t aLen -> c_in:carry t -> tuple2 (carry t) (lbignum t aLen)
+let bn_sub_carry #t #aLen a c_in = generate_elems aLen aLen (bn_sub_carry_f a) c_in
 
 val bn_sub_f: #t:limb_t -> #aLen:size_nat -> a:lbignum t aLen -> b:lbignum t aLen -> i:size_nat{i < aLen} -> c:carry t -> carry t & limb t
 let bn_sub_f #t #aLen a b i c = subborrow c a.[i] b.[i]
@@ -26,16 +26,26 @@ let bn_sub #t #aLen #bLen a b =
   let c0, res0 = generate_elems bLen bLen (bn_sub_f (sub a 0 bLen) b) (uint #t 0) in
 
   if bLen < aLen then
-    let c1, res1 = bn_sub1 (sub a bLen (aLen - bLen)) c0 in
+    let c1, res1 = bn_sub_carry (sub a bLen (aLen - bLen)) c0 in
     c1, concat #_ #bLen res0 res1
   else c0, res0
 
+val bn_sub1: #t:limb_t -> #aLen:size_pos -> a:lbignum t aLen -> b1:limb t -> tuple2 (carry t) (lbignum t aLen)
+let bn_sub1 #t #aLen a b1 =
+  let c0, r0 = subborrow (uint #t 0) a.[0] b1 in
+  let res0 = create 1 r0 in
 
-val bn_add1_f: #t:limb_t -> #aLen:size_nat -> a:lbignum t aLen -> i:size_nat{i < aLen} -> c_in:carry t -> carry t & limb t
-let bn_add1_f #t #aLen a i c_in = addcarry c_in a.[i] (uint #t 0)
+  if 1 < aLen then
+    let c1, res1 = bn_sub_carry (sub a 1 (aLen - 1)) c0 in
+    c1, concat res0 res1
+  else c0, res0
 
-val bn_add1: #t:limb_t -> #aLen:size_nat -> a:lbignum t aLen -> c_in:carry t -> tuple2 (carry t) (lbignum t aLen)
-let bn_add1 #t #aLen a c_in = generate_elems aLen aLen (bn_add1_f a) c_in
+
+val bn_add_carry_f: #t:limb_t -> #aLen:size_nat -> a:lbignum t aLen -> i:size_nat{i < aLen} -> c_in:carry t -> carry t & limb t
+let bn_add_carry_f #t #aLen a i c_in = addcarry c_in a.[i] (uint #t 0)
+
+val bn_add_carry: #t:limb_t -> #aLen:size_nat -> a:lbignum t aLen -> c_in:carry t -> tuple2 (carry t) (lbignum t aLen)
+let bn_add_carry #t #aLen a c_in = generate_elems aLen aLen (bn_add_carry_f a) c_in
 
 val bn_add_f: #t:limb_t -> #aLen:size_nat -> a:lbignum t aLen -> b:lbignum t aLen -> i:size_nat{i < aLen} -> c:carry t -> carry t & limb t
 let bn_add_f #t #aLen a b i c = addcarry c a.[i] b.[i]
@@ -45,12 +55,22 @@ let bn_add #t #aLen #bLen a b =
   let c0, res0 = generate_elems bLen bLen (bn_add_f (sub a 0 bLen) b) (uint #t 0) in
 
   if bLen < aLen then
-    let c1, res1 = bn_add1 (sub a bLen (aLen - bLen)) c0 in
+    let c1, res1 = bn_add_carry (sub a bLen (aLen - bLen)) c0 in
     c1, concat #_ #bLen res0 res1
   else c0, res0
 
+val bn_add1: #t:limb_t -> #aLen:size_pos -> a:lbignum t aLen -> b1:limb t -> tuple2 (carry t) (lbignum t aLen)
+let bn_add1 #t #aLen a b1 =
+  let c0, r0 = addcarry (uint #t 0) a.[0] b1 in
+  let res0 = create 1 r0 in
 
-val bn_add1_lemma_loop_step:
+  if 1 < aLen then
+    let c1, res1 = bn_add_carry (sub a 1 (aLen - 1)) c0 in
+    c1, concat res0 res1
+  else c0, res0
+
+
+val bn_add_carry_lemma_loop_step:
     #t:limb_t
   -> #aLen:size_nat
   -> a:lbignum t aLen
@@ -61,12 +81,12 @@ val bn_add1_lemma_loop_step:
    (let (c1, res1) = c1_res1 in
     v c1 * pow2 (bits t * (i - 1)) + bn_v #t #(i - 1) res1 == eval_ aLen a (i - 1) + v c_in))
   (ensures
-   (let (c_out, res) = generate_elem_f aLen (bn_add1_f a) (i - 1) c1_res1 in
+   (let (c_out, res) = generate_elem_f aLen (bn_add_carry_f a) (i - 1) c1_res1 in
     v c_out * pow2 (bits t * i) + bn_v #t #i res == eval_ aLen a i + v c_in))
 
-let bn_add1_lemma_loop_step #t #aLen a c_in i (c1, res1) =
-  let (c_out, res) = generate_elem_f aLen (bn_add1_f a) (i - 1) (c1, res1) in
-  let c, e = bn_add1_f a (i - 1) c1 in
+let bn_add_carry_lemma_loop_step #t #aLen a c_in i (c1, res1) =
+  let (c_out, res) = generate_elem_f aLen (bn_add_carry_f a) (i - 1) (c1, res1) in
+  let c, e = bn_add_carry_f a (i - 1) c1 in
   assert (v e + v c * pow2 (bits t) == v a.[i - 1] + v c1);
   let pbits = bits t in
 
@@ -88,45 +108,45 @@ let bn_add1_lemma_loop_step #t #aLen a c_in i (c1, res1) =
   assert (v c * pow2 (pbits * i) + bn_v #t #i res == eval_ aLen a i + v c_in)
 
 
-val bn_add1_lemma_loop:
+val bn_add_carry_lemma_loop:
     #t:limb_t
   -> #aLen:size_nat
   -> a:lbignum t aLen
   -> c_in:carry t
   -> i:nat{i <= aLen} ->
-  Lemma (let (c_out, res) : generate_elem_a (limb t) (carry t) aLen i = generate_elems aLen i (bn_add1_f a) c_in in
+  Lemma (let (c_out, res) : generate_elem_a (limb t) (carry t) aLen i = generate_elems aLen i (bn_add_carry_f a) c_in in
    v c_out * pow2 (bits t * i) + bn_v #t #i res == eval_ aLen a i + v c_in)
 
-let rec bn_add1_lemma_loop #t #aLen a c_in i =
+let rec bn_add_carry_lemma_loop #t #aLen a c_in i =
   let pbits = bits t in
-  let (c_out, res) : generate_elem_a (limb t) (carry t) aLen i = generate_elems aLen i (bn_add1_f a) c_in in
+  let (c_out, res) : generate_elem_a (limb t) (carry t) aLen i = generate_elems aLen i (bn_add_carry_f a) c_in in
   if i = 0 then begin
-    eq_generate_elems0 aLen i (bn_add1_f a) c_in;
+    eq_generate_elems0 aLen i (bn_add_carry_f a) c_in;
     assert (c_out == c_in /\ res == Seq.empty);
     bn_eval0 #t #0 res;
     assert_norm (pow2 0 = 1);
     bn_eval0 a;
     () end
   else begin
-    let (c1, res1) : generate_elem_a (limb t) (carry t) aLen (i - 1) = generate_elems aLen (i - 1) (bn_add1_f a) c_in in
-    generate_elems_unfold aLen i (bn_add1_f a) c_in (i - 1);
-    assert (generate_elems aLen i (bn_add1_f a) c_in ==
-      generate_elem_f aLen (bn_add1_f a) (i - 1) (generate_elems aLen (i - 1) (bn_add1_f a) c_in));
-    assert ((c_out, res) == generate_elem_f aLen (bn_add1_f a) (i - 1) (c1, res1));
-    bn_add1_lemma_loop a c_in (i - 1);
+    let (c1, res1) : generate_elem_a (limb t) (carry t) aLen (i - 1) = generate_elems aLen (i - 1) (bn_add_carry_f a) c_in in
+    generate_elems_unfold aLen i (bn_add_carry_f a) c_in (i - 1);
+    assert (generate_elems aLen i (bn_add_carry_f a) c_in ==
+      generate_elem_f aLen (bn_add_carry_f a) (i - 1) (generate_elems aLen (i - 1) (bn_add_carry_f a) c_in));
+    assert ((c_out, res) == generate_elem_f aLen (bn_add_carry_f a) (i - 1) (c1, res1));
+    bn_add_carry_lemma_loop a c_in (i - 1);
     assert (v c1 * pow2 (pbits * (i - 1)) + bn_v #t #(i - 1) res1 == eval_ aLen a (i - 1) + v c_in);
-    bn_add1_lemma_loop_step a c_in i (c1, res1);
+    bn_add_carry_lemma_loop_step a c_in i (c1, res1);
     assert (v c_out * pow2 (pbits * i) + bn_v #t #i res == eval_ aLen a i + v c_in);
     () end
 
 
-val bn_add1_lemma: #t:limb_t -> #aLen:size_nat -> a:lbignum t aLen -> c_in:carry t ->
-  Lemma (let (c_out, res) = bn_add1 a c_in in
+val bn_add_carry_lemma: #t:limb_t -> #aLen:size_nat -> a:lbignum t aLen -> c_in:carry t ->
+  Lemma (let (c_out, res) = bn_add_carry a c_in in
    v c_out * pow2 (bits t * aLen) + bn_v res == bn_v a + v c_in)
 
-let bn_add1_lemma #t #aLen a c_in =
-  let (c_out, res) = bn_add1 a c_in in
-  bn_add1_lemma_loop a c_in aLen
+let bn_add_carry_lemma #t #aLen a c_in =
+  let (c_out, res) = bn_add_carry a c_in in
+  bn_add_carry_lemma_loop a c_in aLen
 
 
 val bn_add_lemma_loop_step:
@@ -205,6 +225,50 @@ let rec bn_add_lemma_loop #t #aLen a b i =
     () end
 
 
+val bn_add_concat_lemma:
+    #t:limb_t
+  -> #aLen:size_nat
+  -> #bLen:size_nat{bLen < aLen}
+  -> a:lbignum t aLen
+  -> b:lbignum t bLen
+  -> c0:carry t
+  -> res0:lbignum t bLen -> Lemma
+  (requires
+    v c0 * pow2 (bits t * bLen) + bn_v #t #bLen res0 == eval_ bLen (sub a 0 bLen) bLen + eval_ bLen b bLen)
+  (ensures
+   (let c1, res1 = bn_add_carry (sub a bLen (aLen - bLen)) c0 in
+    let res = concat #_ #bLen res0 res1 in
+    bn_v res == eval_ aLen a aLen + eval_ bLen b bLen - v c1 * pow2 (bits t * aLen)))
+
+let bn_add_concat_lemma #t #aLen #bLen a b c0 res0 =
+  let pbits = bits t in
+  let a0 = sub a 0 bLen in
+  let a1 = sub a bLen (aLen - bLen) in
+
+  let c1, res1 = bn_add_carry a1 c0 in
+  bn_add_carry_lemma a1 c0;
+  assert (v c1 * pow2 (pbits * (aLen - bLen)) + bn_v res1 == bn_v a1 + v c0);
+
+  let res = concat #_ #bLen res0 res1 in
+  eq_intro (slice res 0 bLen) res0;
+  eq_intro (slice res bLen aLen) res1;
+  bn_eval_split_i res bLen;
+  assert (bn_v res == bn_v #t #bLen res0 + pow2 (pbits * bLen) * bn_v res1);
+  calc (==) {
+    bn_v #t #bLen res0 + pow2 (pbits * bLen) * bn_v res1;
+    (==) { }
+    eval_ bLen a0 bLen + eval_ bLen b bLen - v c0 * pow2 (pbits * bLen) + pow2 (pbits * bLen) * (bn_v a1 + v c0 - v c1 * pow2 (pbits * (aLen - bLen)));
+    (==) { Math.Lemmas.distributivity_sub_right (pow2 (pbits * bLen)) (bn_v a1 + v c0) (v c1 * pow2 (pbits * (aLen - bLen))) }
+    eval_ bLen a0 bLen + eval_ bLen b bLen - v c0 * pow2 (pbits * bLen) + pow2 (pbits * bLen) * (bn_v a1 + v c0) - pow2 (pbits * bLen) * v c1 * pow2 (pbits * (aLen - bLen));
+    (==) { Math.Lemmas.paren_mul_right (pow2 (pbits * bLen)) (v c1) (pow2 (pbits * (aLen - bLen))); Math.Lemmas.pow2_plus (pbits * bLen) (pbits * (aLen - bLen)) }
+    eval_ bLen a0 bLen + eval_ bLen b bLen - v c0 * pow2 (pbits * bLen) + pow2 (pbits * bLen) * (bn_v a1 + v c0) - v c1 * pow2 (pbits * aLen);
+    (==) { Math.Lemmas.distributivity_sub_right (pow2 (pbits * bLen)) (bn_v a1) (v c0) }
+    eval_ bLen a0 bLen + eval_ bLen b bLen + pow2 (pbits * bLen) * bn_v a1 - v c1 * pow2 (pbits * aLen);
+    (==) { bn_eval_split_i a bLen; bn_eval_extensionality_j a (sub a 0 bLen) bLen }
+    eval_ aLen a aLen + eval_ bLen b bLen - v c1 * pow2 (pbits * aLen);
+  }
+
+
 val bn_add_lemma:
     #t:limb_t
   -> #aLen:size_nat
@@ -226,30 +290,39 @@ let bn_add_lemma #t #aLen #bLen a b =
     let c0, res0 = generate_elems bLen bLen (bn_add_f a0 b) (uint #t 0) in
     bn_add_lemma_loop a0 b bLen;
     assert (v c0 * pow2 (pbits * bLen) + bn_v #t #bLen res0 == eval_ bLen a0 bLen + eval_ bLen b bLen);
-    let c1, res1 = bn_add1 a1 c0 in
-    bn_add1_lemma a1 c0;
-    assert (v c1 * pow2 (pbits * (aLen - bLen)) + bn_v res1 == bn_v a1 + v c0);
-    let res = concat #_ #bLen res0 res1 in
-    eq_intro (slice res 0 bLen) res0;
-    eq_intro (slice res bLen aLen) res1;
-    bn_eval_split_i res bLen;
-    assert (bn_v res == bn_v #t #bLen res0 + pow2 (pbits * bLen) * bn_v res1);
-    calc (==) {
-      bn_v #t #bLen res0 + pow2 (pbits * bLen) * bn_v res1;
-      (==) { }
-      eval_ bLen a0 bLen + eval_ bLen b bLen - v c0 * pow2 (pbits * bLen) + pow2 (pbits * bLen) * (bn_v a1 + v c0 - v c1 * pow2 (pbits * (aLen - bLen)));
-      (==) { Math.Lemmas.distributivity_sub_right (pow2 (pbits * bLen)) (bn_v a1 + v c0) (v c1 * pow2 (pbits * (aLen - bLen))) }
-      eval_ bLen a0 bLen + eval_ bLen b bLen - v c0 * pow2 (pbits * bLen) + pow2 (pbits * bLen) * (bn_v a1 + v c0) - pow2 (pbits * bLen) * v c1 * pow2 (pbits * (aLen - bLen));
-      (==) { Math.Lemmas.paren_mul_right (pow2 (pbits * bLen)) (v c1) (pow2 (pbits * (aLen - bLen))); Math.Lemmas.pow2_plus (pbits * bLen) (pbits * (aLen - bLen)) }
-      eval_ bLen a0 bLen + eval_ bLen b bLen - v c0 * pow2 (pbits * bLen) + pow2 (pbits * bLen) * (bn_v a1 + v c0) - v c1 * pow2 (pbits * aLen);
-      (==) { Math.Lemmas.distributivity_sub_right (pow2 (pbits * bLen)) (bn_v a1) (v c0) }
-      eval_ bLen a0 bLen + eval_ bLen b bLen + pow2 (pbits * bLen) * bn_v a1 - v c1 * pow2 (pbits * aLen);
-      (==) { bn_eval_split_i a bLen; bn_eval_extensionality_j a (sub a 0 bLen) bLen }
-      eval_ aLen a aLen + eval_ bLen b bLen  - v c1 * pow2 (pbits * aLen);
-    }; () end
+    bn_add_concat_lemma #t #aLen #bLen a b c0 res0 end
 
 
-val bn_sub1_lemma_loop_step:
+val bn_add1_lemma:
+    #t:limb_t
+  -> #aLen:size_pos
+  -> a:lbignum t aLen
+  -> b1:limb t ->
+  Lemma (let (c, res) = bn_add1 a b1 in
+   v c * pow2 (bits t * aLen) + bn_v res == bn_v a + v b1)
+
+let bn_add1_lemma #t #aLen a b1 =
+  let pbits = bits t in
+  let c0, r0 = addcarry (uint #t 0) a.[0] b1 in
+  assert (v c0 * pow2 pbits + v r0 = v a.[0] + v b1);
+
+  let res0 = create 1 r0 in
+  let b = create 1 b1 in
+  bn_eval1 res0;
+  bn_eval1 b;
+
+  if aLen = 1 then
+    bn_eval1 a
+  else begin
+    let bLen = 1 in
+    let a0 = sub a 0 bLen in
+    bn_eval1 a0;
+    assert (v c0 * pow2 (pbits * bLen) + bn_v #t #1 res0 == eval_ bLen a0 bLen + eval_ bLen b bLen);
+    bn_add_concat_lemma a b c0 res0 end
+
+
+
+val bn_sub_carry_lemma_loop_step:
     #t:limb_t
   -> #aLen:size_nat
   -> a:lbignum t aLen
@@ -260,13 +333,13 @@ val bn_sub1_lemma_loop_step:
    (let (c1, res1) = c1_res1 in
     bn_v #t #(i - 1) res1 - v c1 * pow2 (bits t * (i - 1)) == eval_ aLen a (i - 1) - v c_in))
   (ensures
-   (let (c_out, res) = generate_elem_f aLen (bn_sub1_f a) (i - 1) c1_res1 in
+   (let (c_out, res) = generate_elem_f aLen (bn_sub_carry_f a) (i - 1) c1_res1 in
     bn_v #t #i res - v c_out * pow2 (bits t * i) == eval_ aLen a i - v c_in))
 
-let bn_sub1_lemma_loop_step #t #aLen a c_in i (c1, res1) =
+let bn_sub_carry_lemma_loop_step #t #aLen a c_in i (c1, res1) =
   let pbits = bits t in
-  let (c_out, res) = generate_elem_f aLen (bn_sub1_f a) (i - 1) (c1, res1) in
-  let c, e = bn_sub1_f a (i - 1) c1 in
+  let (c_out, res) = generate_elem_f aLen (bn_sub_carry_f a) (i - 1) (c1, res1) in
+  let c, e = bn_sub_carry_f a (i - 1) c1 in
   assert (v e - v c * pow2 pbits == v a.[i - 1] - v c1);
 
   calc (==) {
@@ -287,45 +360,45 @@ let bn_sub1_lemma_loop_step #t #aLen a c_in i (c1, res1) =
   assert (bn_v #t #i res - v c * pow2 (pbits * i) == eval_ aLen a i - v c_in)
 
 
-val bn_sub1_lemma_loop:
+val bn_sub_carry_lemma_loop:
     #t:limb_t
   -> #aLen:size_nat
   -> a:lbignum t aLen
   -> c_in:carry t
   -> i:nat{i <= aLen} ->
-  Lemma (let (c_out, res) : generate_elem_a (limb t) (carry t) aLen i = generate_elems aLen i (bn_sub1_f a) c_in in
+  Lemma (let (c_out, res) : generate_elem_a (limb t) (carry t) aLen i = generate_elems aLen i (bn_sub_carry_f a) c_in in
    bn_v #t #i res - v c_out * pow2 (bits t * i) == eval_ aLen a i - v c_in)
 
-let rec bn_sub1_lemma_loop #t #aLen a c_in i =
+let rec bn_sub_carry_lemma_loop #t #aLen a c_in i =
   let pbits = bits t in
-  let (c_out, res) : generate_elem_a (limb t) (carry t) aLen i = generate_elems aLen i (bn_sub1_f a) c_in in
+  let (c_out, res) : generate_elem_a (limb t) (carry t) aLen i = generate_elems aLen i (bn_sub_carry_f a) c_in in
   if i = 0 then begin
-    eq_generate_elems0  aLen i (bn_sub1_f a) c_in;
+    eq_generate_elems0  aLen i (bn_sub_carry_f a) c_in;
     assert (c_out == c_in /\ res == Seq.empty);
     bn_eval0 #t #0 res;
     assert_norm (pow2 0 = 1);
     bn_eval0 a;
     () end
   else begin
-    let (c1, res1) : generate_elem_a (limb t) (carry t) aLen (i - 1) = generate_elems aLen (i - 1) (bn_sub1_f a) c_in in
-    generate_elems_unfold aLen i (bn_sub1_f a) c_in (i - 1);
-    assert (generate_elems aLen i (bn_sub1_f a) c_in ==
-      generate_elem_f aLen (bn_sub1_f a) (i - 1) (generate_elems aLen (i - 1) (bn_sub1_f a) c_in));
-    assert ((c_out, res) == generate_elem_f  aLen (bn_sub1_f a) (i - 1) (c1, res1));
-    bn_sub1_lemma_loop a c_in (i - 1);
+    let (c1, res1) : generate_elem_a (limb t) (carry t) aLen (i - 1) = generate_elems aLen (i - 1) (bn_sub_carry_f a) c_in in
+    generate_elems_unfold aLen i (bn_sub_carry_f a) c_in (i - 1);
+    assert (generate_elems aLen i (bn_sub_carry_f a) c_in ==
+      generate_elem_f aLen (bn_sub_carry_f a) (i - 1) (generate_elems aLen (i - 1) (bn_sub_carry_f a) c_in));
+    assert ((c_out, res) == generate_elem_f  aLen (bn_sub_carry_f a) (i - 1) (c1, res1));
+    bn_sub_carry_lemma_loop a c_in (i - 1);
     assert (bn_v #t #(i - 1) res1 - v c1 * pow2 (pbits * (i - 1)) == eval_ aLen a (i - 1) - v c_in);
-    bn_sub1_lemma_loop_step a c_in i (c1, res1);
+    bn_sub_carry_lemma_loop_step a c_in i (c1, res1);
     assert (bn_v #t #i res - v c_out * pow2 (pbits * i) == eval_ aLen a i - v c_in);
     () end
 
 
-val bn_sub1_lemma: #t:limb_t -> #aLen:size_nat -> a:lbignum t aLen -> c_in:carry t ->
-  Lemma (let (c_out, res) = bn_sub1 a c_in in
+val bn_sub_carry_lemma: #t:limb_t -> #aLen:size_nat -> a:lbignum t aLen -> c_in:carry t ->
+  Lemma (let (c_out, res) = bn_sub_carry a c_in in
    bn_v res - v c_out * pow2 (bits t * aLen) == bn_v a - v c_in)
 
-let bn_sub1_lemma #t #aLen a c_in =
-  let (c_out, res) = bn_sub1 a c_in in
-  bn_sub1_lemma_loop a c_in aLen
+let bn_sub_carry_lemma #t #aLen a c_in =
+  let (c_out, res) = bn_sub_carry a c_in in
+  bn_sub_carry_lemma_loop a c_in aLen
 
 
 val bn_sub_lemma_loop_step:
@@ -402,6 +475,50 @@ let rec bn_sub_lemma_loop #t #aLen a b i =
     () end
 
 
+val bn_sub_concat_lemma:
+    #t:limb_t
+  -> #aLen:size_nat
+  -> #bLen:size_nat{bLen < aLen}
+  -> a:lbignum t aLen
+  -> b:lbignum t bLen
+  -> c0:carry t
+  -> res0:lbignum t bLen -> Lemma
+  (requires
+    bn_v #t #bLen res0 - v c0 * pow2 (bits t * bLen) == eval_ bLen (sub a 0 bLen) bLen - eval_ bLen b bLen)
+  (ensures
+   (let c1, res1 = bn_sub_carry (sub a bLen (aLen - bLen)) c0 in
+    let res = concat #_ #bLen res0 res1 in
+    bn_v res == eval_ aLen a aLen - eval_ bLen b bLen + v c1 * pow2 (bits t * aLen)))
+
+let bn_sub_concat_lemma #t #aLen #bLen a b c0 res0 =
+  let pbits = bits t in
+  let a0 = sub a 0 bLen in
+  let a1 = sub a bLen (aLen - bLen) in
+
+  let c1, res1 = bn_sub_carry a1 c0 in
+  bn_sub_carry_lemma a1 c0;
+  assert (bn_v res1 - v c1 * pow2 (pbits * (aLen - bLen)) == bn_v a1 - v c0);
+
+  let res = concat #_ #bLen res0 res1 in
+  eq_intro (slice res 0 bLen) res0;
+  eq_intro (slice res bLen aLen) res1;
+  bn_eval_split_i res bLen;
+  assert (bn_v res == bn_v #t #bLen res0 + pow2 (pbits * bLen) * bn_v res1);
+  calc (==) {
+    bn_v #t #bLen res0 + pow2 (pbits * bLen) * bn_v res1;
+    (==) { }
+    eval_ bLen a0 bLen - eval_ bLen b bLen + v c0 * pow2 (pbits * bLen) + pow2 (pbits * bLen) * (bn_v a1 - v c0 + v c1 * pow2 (pbits * (aLen - bLen)));
+    (==) { Math.Lemmas.distributivity_sub_right (pow2 (pbits * bLen)) (bn_v a1 + v c1 * pow2 (pbits * (aLen - bLen))) (v c0) }
+    eval_ bLen a0 bLen - eval_ bLen b bLen + v c0 * pow2 (pbits * bLen) + pow2 (pbits * bLen) * (bn_v a1 + v c1 * pow2 (pbits * (aLen - bLen))) - pow2 (pbits * bLen) * v c0;
+    (==) { Math.Lemmas.distributivity_add_right (pow2 (pbits * bLen)) (bn_v a1) (v c1 * pow2 (pbits * (aLen - bLen))) }
+    eval_ bLen a0 bLen - eval_ bLen b bLen + pow2 (pbits * bLen) * bn_v a1 + pow2 (pbits * bLen) * v c1 * pow2 (pbits * (aLen - bLen));
+    (==) { Math.Lemmas.paren_mul_right (pow2 (pbits * bLen)) (v c1) (pow2 (pbits * (aLen - bLen))); Math.Lemmas.pow2_plus (pbits * bLen) (pbits * (aLen - bLen)) }
+    eval_ bLen a0 bLen - eval_ bLen b bLen + pow2 (pbits * bLen) * bn_v a1 + v c1 * pow2 (pbits * aLen);
+    (==) { bn_eval_split_i a bLen; bn_eval_extensionality_j a (sub a 0 bLen) bLen }
+    eval_ aLen a aLen - eval_ bLen b bLen + v c1 * pow2 (pbits * aLen);
+  }
+
+
 val bn_sub_lemma:
     #t:limb_t
   -> #aLen:size_nat
@@ -423,24 +540,32 @@ let bn_sub_lemma #t #aLen #bLen a b =
     let c0, res0 = generate_elems bLen bLen (bn_sub_f a0 b) (uint #t 0) in
     bn_sub_lemma_loop a0 b bLen;
     assert (bn_v #t #bLen res0 - v c0 * pow2 (pbits * bLen) == eval_ bLen a0 bLen - eval_ bLen b bLen);
-    let c1, res1 = bn_sub1 a1 c0 in
-    bn_sub1_lemma a1 c0;
-    assert (bn_v res1 - v c1 * pow2 (pbits * (aLen - bLen)) == bn_v a1 - v c0);
-    let res = concat #_ #bLen res0 res1 in
-    eq_intro (slice res 0 bLen) res0;
-    eq_intro (slice res bLen aLen) res1;
-    bn_eval_split_i res bLen;
-    assert (bn_v res == bn_v #t #bLen res0 + pow2 (pbits * bLen) * bn_v res1);
-    calc (==) {
-      bn_v #t #bLen res0 + pow2 (pbits * bLen) * bn_v res1;
-      (==) { }
-      eval_ bLen a0 bLen - eval_ bLen b bLen + v c0 * pow2 (pbits * bLen) + pow2 (pbits * bLen) * (bn_v a1 - v c0 + v c1 * pow2 (pbits * (aLen - bLen)));
-      (==) { Math.Lemmas.distributivity_sub_right (pow2 (pbits * bLen)) (bn_v a1 + v c1 * pow2 (pbits * (aLen - bLen))) (v c0) }
-      eval_ bLen a0 bLen - eval_ bLen b bLen + v c0 * pow2 (pbits * bLen) + pow2 (pbits * bLen) * (bn_v a1 + v c1 * pow2 (pbits * (aLen - bLen))) - pow2 (pbits * bLen) * v c0;
-      (==) { Math.Lemmas.distributivity_add_right (pow2 (pbits * bLen)) (bn_v a1) (v c1 * pow2 (pbits * (aLen - bLen))) }
-      eval_ bLen a0 bLen - eval_ bLen b bLen + pow2 (pbits * bLen) * bn_v a1 + pow2 (pbits * bLen) * v c1 * pow2 (pbits * (aLen - bLen));
-      (==) { Math.Lemmas.paren_mul_right (pow2 (pbits * bLen)) (v c1) (pow2 (pbits * (aLen - bLen))); Math.Lemmas.pow2_plus (pbits * bLen) (pbits * (aLen - bLen)) }
-      eval_ bLen a0 bLen - eval_ bLen b bLen + pow2 (pbits * bLen) * bn_v a1 + v c1 * pow2 (pbits * aLen);
-      (==) { bn_eval_split_i a bLen; bn_eval_extensionality_j a (sub a 0 bLen) bLen }
-      eval_ aLen a aLen - eval_ bLen b bLen + v c1 * pow2 (pbits * aLen);
-    }; () end
+    bn_sub_concat_lemma #t #aLen #bLen a b c0 res0 end
+
+
+val bn_sub1_lemma:
+    #t:limb_t
+  -> #aLen:size_pos
+  -> a:lbignum t aLen
+  -> b1:limb t ->
+  Lemma (let (c, res) = bn_sub1 a b1 in
+    bn_v res - v c * pow2 (bits t * aLen) == bn_v a - v b1)
+
+let bn_sub1_lemma #t #aLen a b1 =
+  let pbits = bits t in
+  let c0, r0 = subborrow (uint #t 0) a.[0] b1 in
+  assert (v r0 - v c0 * pow2 pbits = v a.[0] - v b1);
+
+  let res0 = create 1 r0 in
+  let b = create 1 b1 in
+  bn_eval1 res0;
+  bn_eval1 b;
+
+  if aLen = 1 then
+    bn_eval1 a
+  else begin
+    let bLen = 1 in
+    let a0 = sub a 0 bLen in
+    bn_eval1 a0;
+    assert (bn_v #t #1 res0 - v c0 * pow2 (pbits * bLen) == eval_ bLen a0 bLen - eval_ bLen b bLen);
+    bn_sub_concat_lemma a b c0 res0 end
